

标题

啊波吡

2024 年 10 月 12 日

目录

先解不等式 $x^2 - (2a + 2)x + 2a < 0$.

令 $x^2 - (2a + 2)x + 2a = 0$. 由求根公式得

$$x = a + 1 \pm \sqrt{a^2 + a}.$$

所以

$$\text{左边} = x^2 - (2a + 2)x + 2a = (x - (a + 1 + \sqrt{a^2 + a}))(x - (a + 1 - \sqrt{a^2 + a})).$$

于是原不等式等价于

$$(x - (a + 1 + \sqrt{a^2 + a}))(x - (a + 1 - \sqrt{a^2 + a})) < 0.$$

因为 $(a + 1 - \sqrt{a^2 + a}) < (a + 1 + \sqrt{a^2 + a})$, 所以原不等式的解集为

$$a + 1 - \sqrt{a^2 + a} < x < a + 1 + \sqrt{a^2 + a}.$$

由该不等式有且只有三个整数解, 可知

$$4 < 2a + 1 \leq 5.$$

解得 a